lean/src/a_eval_theorem.lean
@@ -1,11 +1,352 @@
+import tactic
 import .defs
+import .lemmas
 
 variable [GuardModule]
 open GuardModule
+
+lemma foo (ant: Ant Φ) (ty: Φ) (env: Env):
+    ant_eval (map_ant (ty.and) ant) env
+    = ant_eval' (map_ant (band (Φ_eval ty env)) (ant_eval_all ant env)) :=
+begin
+    sorry
+end
+
+-- for the sake of lean, it must be possible to simplify this drastically.
+lemma and_no_match (ant: Ant Φ) (ty: Φ) (env: Env):
+    ant_eval ant env = some Result.no_match
+    → ant_eval (map_ant (ty.and) ant) env = some Result.no_match :=
+begin
+    assume h,
+    rw ant_eval,
+    rw ant_eval_all,
+    
+    induction ant,
+
+    case Ant.leaf {
+        rw ant_eval at h,
+        rw ant_eval_all at h,
+        rw map_ant at h,
+        rw ant_eval' at h,
+        cases c: Φ_eval ant_a env,
+        all_goals {
+            rw c at h,
+            simp at h,
+        },
+        case bool.tt {
+            cc,
+        },
+        rw map_ant,
+        rw map_ant,
+        rw ant_eval',
+        rw Φ_eval,
+        finish,
+    },
+
+    case Ant.branch {
+        rw ant_eval at h,
+        rw ant_eval_all at h,
+        rw map_ant at h,
+        rw ←ant_eval_all at h,
+        rw ←ant_eval_all at h,
+        rw ant_eval' at h,
+        
+        
+        rw ←ant_eval at h,
+        rw ←ant_eval at h,
+
+        rw map_ant,
+        rw map_ant,
+        rw ant_eval',
+
+        by_cases c1: (ant_eval ant_tr1 env = some Result.no_match),
+        all_goals {
+            by_cases c2: (ant_eval ant_tr2 env = some Result.no_match),
+        },
+
+        {
+            cc,
+        },
+        {
+            rw c1 at ant_ih_tr1,
+            rw c1 at h,
+            simp at ant_ih_tr1,
+            rw ant_ih_tr1,
+            
+            cases ant_eval ant_tr2 env,
+            case option.none {
+                rw ant_eval'._match_1 at h,
+                cc,
+            },
+            case option.some {
+                cases val,
+                all_goals {
+                    rw ant_eval'._match_1 at h,
+                    cc,
+                },
+            },
+        },
+        {
+            rw c2 at ant_ih_tr2,
+            rw c2 at h,
+            simp at ant_ih_tr2,
+            rw ant_ih_tr2,
+            cases ant_eval ant_tr1 env,
+            case option.none {
+                rw ant_eval'._match_1 at h,
+                cc,
+            },
+            case option.some {
+                cases val,
+                all_goals {
+                    rw ant_eval'._match_1 at h,
+                    cc,
+                },
+            },
+        },
+        {
+            cases ant_eval ant_tr1 env,
+            all_goals {
+                cases ant_eval ant_tr2 env,
+            },
+            case option.none option.none {
+                rw ant_eval'._match_1 at h,
+                cc,
+            },
+            case option.some option.none {
+                cases val,
+                all_goals {
+                    rw ant_eval'._match_1 at h,
+                    cc,
+                },
+            },
+            case option.none option.some {
+                cases val,
+                all_goals {
+                    rw ant_eval'._match_1 at h,
+                    cc,
+                },
+            },
+            case option.some option.some {
+                cases val,
+                all_goals {
+                    cases val_1,
+                },
+                all_goals {
+                    rw ant_eval'._match_1 at h,
+                    cc,
+                },
+            },
+        },
+    },
+    case Ant.diverge {
+        rw ant_eval at h,
+        rw ant_eval_all at h,
+        rw map_ant at h,
+        rw ant_eval' at h,
+
+        rw map_ant,
+        rw map_ant,
+        rw ant_eval',
+        rw ←ant_eval_all at h,
+        rw ←ant_eval at h,
+
+        have x : ant_eval ant_tr env = some Result.no_match, {
+            cases Φ_eval ant_a env,
+            all_goals {
+                cases ant_eval ant_tr env,
+            },
+            all_goals {
+                try {
+                    cases val,
+                },
+            },
+            case bool.ff option.some Result.leaf {
+                rw ant_eval'._match_2 at h,
+                cc,
+            },
+            case bool.ff option.some Result.diverged {
+                rw ant_eval'._match_2 at h,
+                cc,
+            },
+            all_goals {
+                finish,
+            },
+        },
+
+        rw x at ant_ih,
+        simp at ant_ih,
+        rw ant_ih,
+        cases c: Φ_eval (ty.and ant_a) env,
+        all_goals {
+            rw ant_eval'._match_2,
+        },
+        rw x at h,
+        rw Φ_eval at c,
+        have y: Φ_eval ant_a env = tt, {
+            rw band_eq_true_eq_eq_tt_and_eq_tt at c,
+            exact c.right,
+        },
+        rw y at h,
+        rw ant_eval'._match_2 at h,
+        cc,
+    },
+end
+
+lemma ant_eval_is_some_and (ant: Ant Φ) (env: Env) (ty: Φ):
+    option.is_some (ant_eval ant env)
+    → option.is_some (ant_eval (map_ant (ty.and) ant) env) :=
+begin
+    assume h,
+    induction ant with h2,
+    
+        
+    
+    case Ant.leaf {
+        unfold 𝒜' map_ant ant_eval ant_eval ant_eval_all map_ant ant_eval',
+        cases Φ_eval (ty.and h2) env,
+        all_goals { simp },
+    },
+
+    case Ant.branch {
+        
+        conv at h {
+            rw ant_eval,
+            rw ant_eval_all,
+            rw map_ant,
+            rw ant_eval',
+            rw ← ant_eval_all,
+            rw ← ant_eval_all,
+            rw ←ant_eval,
+            rw ←ant_eval,
+        },
+
+        conv {
+            rw map_ant,
+            rw ant_eval,
+            rw ant_eval_all,
+            rw map_ant,
+            rw ant_eval',
+            rw ← ant_eval_all,
+            rw ← ant_eval_all,
+            rw ←ant_eval,
+            rw ←ant_eval,
+        },
+        
+        
+        by_cases h_1: (ant_eval ant_tr1 env = some Result.no_match),
+        all_goals {
+            by_cases h_2: (ant_eval ant_tr2 env = some Result.no_match),
+        },
+        {
+            rw h_1 at ant_ih_tr1,
+            simp at ant_ih_tr1,
+            rw h_2 at ant_ih_tr2,
+            simp at ant_ih_tr2,
+            rw and_no_match,
+            rw and_no_match,
+            rw ant_eval'._match_1,
+            simp,
+            exact h_2,
+            exact h_1,
+        },
+        
+        
+
+
+        /-
+        conv in (ant_eval (map_ant ty.and (𝒜' (gdt_tr1.branch gdt_tr2))) env).is_some {
+            rw 𝒜',
+            rw map_ant,
+            rw ant_eval,
+            rw ant_eval_all,
+            rw map_ant,
+            rw ant_eval',
+            rw ← ant_eval_all,
+            rw ← ant_eval_all,
+            rw ←ant_eval,
+            rw ←ant_eval,
+        },
+        -/
+        
+        
+        /-
+        rw map_ant at h,
+        rw ← ant_eval_all at h,
+        rw ← ant_eval_all at h,
+
+        rw ant_eval' at h,
+        rw ←ant_eval at h,
+        rw ←ant_eval at h,
+        
+        rw map_ant at h,
+        rw ant_eval' at h,
+        -/
+    },
+end
 
 -- 𝒜 maintains semantics
 -- This theorem implies that ant_eval returns a list of length at most 1.
 -- This means that the refinement types created by 𝒜 are disjoint.
 theorem 𝒜_eval :
     ∀ env: Env, ∀ gdt: Gdt,
-        some (gdt_eval gdt env) = ant_eval (𝒜 gdt) env := sorry
+        some (gdt_eval gdt env) = ant_eval (𝒜 gdt) env :=
+begin
+    assume env,
+    assume gdt,
+    rw 𝒜_𝒜'_equiv,
+    
+    induction gdt with env,
+
+    case Gdt.leaf {
+        sorry,
+        --finish,
+    },
+
+    case Gdt.branch {
+        unfold 𝒜',
+        unfold ant_eval,
+        unfold ant_eval_all,
+        unfold map_ant,
+        rw ←ant_eval_all,
+        rw ←ant_eval_all,
+        unfold ant_eval',
+        rw ←ant_eval,
+        rw ←ant_eval,
+        rw ←gdt_ih_tr1,
+
+
+        cases c: (ant_eval (map_ant (𝒰' gdt_tr1).and (𝒜' gdt_tr2)) env),
+
+        case option.none {
+
+        },
+
+
+
+
+
+        cases (gdt_eval gdt_tr1 env),
+        all_goals {
+            cases (ant_eval (map_ant (𝒰' gdt_tr1).and (𝒜' gdt_tr2)) env),
+        },
+        all_goals {
+            try {
+                cases val,
+            },
+        },
+
+        all_goals {
+            unfold ant_eval'._match_1,
+        },
+        repeat {
+            simp,
+        },
+
+        
+        
+        unfold gdt_eval,
+
+    },
+
+end
